Proved preservation

src/SystemT.v
@@ -1,8 +1,25 @@
 Load Maps.
 
+Lemma symmetry_neq : forall {T : Type} (P Q : T), P <> Q <-> Q <> P.
+Proof.
+  intros P Q. split; intros Hneq Heq; subst; apply Hneq; reflexivity.
+Qed.
+
+
+Lemma update_split_shadow: forall T (Gamma : partial_map T) x y a b c,
+        update (update (update Gamma x a) y b) x c =
+        update (update Gamma y b) x c.
+Proof with auto.
+  intros T Gamma x y a b c.
+  apply functional_extensionality. intros z.
+  unfold update. unfold t_update.
+  destruct (beq_idP x z); subst...
+Qed.
+
 Inductive ty : Type :=
   | TNat : ty
   | TArrow : ty -> ty -> ty.
+Hint Constructors ty.
 
 Inductive exp : Type :=
   | Var : id -> exp
@@ -11,8 +28,31 @@ Inductive exp : Type :=
   | Rec : exp -> id -> id -> exp -> exp -> exp
   | Abs : id -> ty -> exp -> exp
   | App : exp -> exp -> exp.
+Hint Constructors exp.
 
 Definition env : Type := partial_map ty.
+
+Inductive appears_free_in : id -> exp -> Prop :=
+  | Afi_Var : forall x, appears_free_in x (Var x)
+  | Afi_S : forall x e, appears_free_in x e -> appears_free_in x (S e)
+  | Afi_App1 : forall x e1 e2,
+      appears_free_in x e1 -> appears_free_in x (App e1 e2)
+  | Afi_App2 : forall x e1 e2,
+      appears_free_in x e2 -> appears_free_in x (App e1 e2)
+  | Afi_Abs : forall x y t e,
+      x <> y -> appears_free_in x e ->
+      appears_free_in x (Abs y t e)
+  | Afi_Rec : forall x y z e0 e1 e,
+      appears_free_in z e -> appears_free_in z (Rec e0 x y e1 e)
+  | Afi_RecZ : forall z e0 x y e1 e,
+      appears_free_in z e0 -> appears_free_in z (Rec e0 x y e1 e)
+  | Afi_RecS : forall z e0 x y e1 e,
+      x <> z -> y <> z -> appears_free_in z e1 ->
+      appears_free_in z (Rec e0 x y e1 e).
+Hint Constructors appears_free_in.
+
+Definition closed (e : exp) :=
+  forall x, ~ appears_free_in x e.
 
 
 Reserved Notation "Gamma |- e \in T" (at level 80).
@@ -31,25 +71,186 @@ Inductive has_type : env -> exp -> ty -> Prop :=
               Gamma |- App e1 e2 \in t
   | T_Rec : forall Gamma e0 x y e1 e t,
               Gamma |- e \in TNat -> Gamma |- e0 \in t ->
+              x <> y ->
               (update (update Gamma y t) x TNat) |- e1 \in t ->
               Gamma |- (Rec e0 x y e1 e) \in t
 where "Gamma |- e \in T" := (has_type Gamma e T).
+Hint Constructors has_type.
 
 Inductive value : exp -> Prop :=
   | Val_Z : value Z
   | Val_S : forall n, value n -> value (S n)
-  | Val_Abs : forall t x e, value (Abs x t e).
+  | Val_Abs : forall x t e, value (Abs x t e).
+Hint Constructors value.
+
+Fixpoint subst (z : id) (e' : exp) (e : exp) : exp :=
+  let do_subst := subst z e' in
+  match e with
+  | Var x as v => if beq_id x z then e' else v
+  | Z => Z
+  | S n => S (do_subst n)
+  | Rec e0 x y e1 e =>
+      let e1' := if beq_id x z || beq_id y z then e1 else do_subst e1 in
+      Rec (do_subst e0) x y e1' (do_subst e)
+  | Abs x t e as abs => if beq_id x z then abs else Abs x t (do_subst e)
+  | App e1 e2 => App (do_subst e1) (do_subst e2)
+  end.
+Notation "'[' x ':=' e1 ']' e" := (subst x e1 e) (at level 70).
+
+Reserved Notation "e ==> e'" (at level 75).
+Inductive step : exp -> exp -> Prop :=
+  | S_Succ : forall e e', e ==> e' -> S(e) ==> S(e')
+  | S_App1 : forall e1 e1' e2,
+      e1 ==> e1' -> App e1 e2 ==> App e1' e2
+  | S_App2 : forall e1 e2 e2',
+      value e1 -> e2 ==> e2' -> App e1 e2 ==> App e1 e2'
+  | S_AppAbs : forall e e2 x t,
+      value e2 -> App (Abs x t e) e2 ==> [x := e2] e
+  | S_Rec1 : forall e0 x y e1 e e',
+      e ==> e' -> Rec e0 x y e1 e ==> Rec e0 x y e1 e'
+  | S_RecZ : forall e0 x y e1, Rec e0 x y e1 Z ==> e0
+  | S_RecS : forall e0 x y e1 e,
+      value (S e) -> Rec e0 x y e1 (S e) ==>
+                    [x := e][y := (Rec e0 x y e1 e)] e1
+where "e ==> e'" := (step e e').
+Hint Constructors step.
+
+Lemma free_in_context : forall x e t Gamma,
+   appears_free_in x e ->
+   Gamma |- e \in t ->
+   exists t', Gamma x = Some t'.
+Proof.
+  intros x e t Gamma Hfree Hte.
+  generalize dependent t. generalize dependent Gamma.
+  induction Hfree; try (intros Gamma t Ht;
+    inversion Ht; subst; clear Ht; eauto).
+  
+  intros Gamma t2 Ht. inversion Ht; subst; clear Ht.
+    apply IHHfree in H5. rewrite update_neq in H5.
+     + assumption.
+     + rewrite symmetry_neq. assumption.
+Qed.
+
+Lemma typable_empty_closed : forall e t,
+    empty |- e \in t  -> closed e.
+Proof.
+  intros e t Hempty x Hfree.
+  apply free_in_context with (t:=t) (Gamma:=empty) in Hfree.
+  - inversion Hfree. inversion H.
+  - assumption.
+Qed.
+
+Lemma weakening : forall Gamma Gamma' e t,
+     Gamma |- e \in t  ->
+     (forall x, appears_free_in x e -> Gamma x = Gamma' x) ->
+     Gamma' |- e \in t.
+Proof with eauto.
+  intros.
+  generalize dependent Gamma'.
+  induction H; intros Gamma' Hfree; auto.
+  - apply T_Var. rewrite <- Hfree...
+  - apply T_Abs. apply IHhas_type. intros x1 Hx1_free.
+    unfold update. unfold t_update. destruct (beq_id x x1) eqn: Heq.
+    + reflexivity.
+    + rewrite beq_id_false_iff in Heq.
+      rewrite Hfree...
+  - apply T_App with t2...
+  - apply T_Rec... apply IHhas_type3. intros x1 Hx1_free.
+    unfold update. unfold t_update.
+    destruct (beq_id x x1) eqn: Heqx...
+    destruct (beq_id y x1) eqn: Heqy...
+    rewrite beq_id_false_iff in Heqx.
+    rewrite beq_id_false_iff in Heqy.
+    apply Hfree. apply Afi_RecS...
+Qed.
 
 Lemma canonical_nat : forall Gamma e,
   value e -> Gamma |- e \in TNat ->
   e = Z \/ exists e', e = (S e').
 Proof.
   intros Gamma e Hv HNat.
-  remember TNat. inversion Hv; subst; clear Hv.
+  inversion Hv; subst; clear Hv.
   - left. reflexivity.
   - right. exists n. reflexivity.
   - inversion HNat.
 Qed.
+
+Lemma canonical_arrow : forall Gamma t1 t2 e,
+  value e -> Gamma |- e \in TArrow t1 t2 ->
+  exists x e2, e = Abs x t1 e2.
+Proof.
+  intros Gamma t1 t2 e Hv Harrow.
+  remember (TArrow t1 t2).
+  inversion Hv; subst; clear Hv.
+  - inversion Harrow.
+  - inversion Harrow.
+  - exists x. exists e0.
+    inversion Harrow; subst; clear Harrow.
+    reflexivity.
+Qed.
+
+Lemma substitution_preserves_typing : forall Gamma e e' t t' x,
+  update Gamma x t |- e' \in t' -> empty |- e \in t ->
+  Gamma |- [x := e] e' \in t'.
+Proof with eauto.
+  intros Gamma e e' t t' x Hte' Hte.
+  generalize dependent Gamma.
+  generalize dependent t'.
+  induction e'; subst; intros t' Gamma H;
+  inversion H; simpl; subst...
+  - rename i into y. destruct (beq_idP y x) as [Hyx|Hyx].
+    + subst.
+      rewrite update_eq in H2. inversion H2; subst.
+      apply weakening with empty. assumption.
+
+      intros y Hy_free.
+      apply typable_empty_closed in Hte. unfold closed in Hte.
+      apply Hte in Hy_free. inversion Hy_free.
+    + apply T_Var. rewrite update_neq in H2.
+      * assumption.
+      * rewrite symmetry_neq. assumption.
+  - rename x into z. rename i into x. rename i0 into y.
+    apply T_Rec...
+    destruct (beq_idP x z) as [Hxz|Hxz]...
+    + subst. simpl. rewrite update_split_shadow in H10...
+    + destruct (beq_idP y z) as [Hyz|Hyz]...
+      * subst. simpl. rewrite update_shadow in H10...
+      * simpl. apply IHe'2.
+        rewrite update_permute...
+        assert (Hhelp: update (update Gamma y t') z t =
+                       update (update Gamma z t) y t').
+        { rewrite update_permute... }
+        rewrite Hhelp...
+  - rename i into y. destruct (beq_idP y x) as [Hyx|Hyx].
+    + subst. apply T_Abs. rewrite update_shadow in H5...
+    + apply T_Abs. apply IHe'. rewrite update_permute...
+Qed.
+
+Lemma preservation : forall e e' t,
+  empty |- e \in t -> e ==> e' -> empty |- e' \in t.
+Proof with eauto.
+  intros e e' t Ht Hstep.
+  generalize dependent e'.
+  remember empty.
+  induction Ht;
+  try solve [subst; intros e' Habsurd; inversion Habsurd; subst; eauto].
+
+  - intros e_appd Hstep. inversion Hstep; subst; clear Hstep...
+    inversion Ht1; subst; clear Ht1.
+    eapply substitution_preserves_typing...
+
+  - intros e_appd Hstep. inversion Hstep; subst; clear Hstep...
+    apply substitution_preserves_typing with (t:=TNat)...
+    + specialize (IHHt1 (eq_refl empty)).
+      specialize (IHHt2 (eq_refl empty)).
+
+      apply substitution_preserves_typing with (t:=t)...
+      * rewrite update_permute...
+      * apply T_Rec...
+        inversion Ht1...
+    + inversion Ht1...
+Qed.
+
 
 
 
